(WIP) geting close to cloning multiple owners without doing it

Klon.dfy
@@ -1,6 +1,7 @@
  
 type Mapping = map<Object,Object>
 
+ 
 ///shoujld thsi be m.KEys or m.ks... 
 predicate OrigMapOK(m : Mapping)
 {
@@ -12,7 +13,6 @@ predicate OrigMapOK(m : Mapping)
   && (forall x <- m.Keys, oo <- x.AMFO :: m[oo] in m[x].AMFO)
 //  && forall x <- m.Keys :: (not(inside(x,o)) ==> (m[x] == x))x
 }
-
 predicate MapOK(m : Mapping)
 {
   && (forall x <- m.Keys, oo <- x.AMFO :: oo in m.Keys)
@@ -21,7 +21,7 @@ predicate MapOK(m : Mapping)
   && (forall x <- m.Keys |  x.region.Heap? :: x.region.owner in m.Keys)
   && (forall x <- m.Keys |  x.region.Heap? :: m[x.region.owner] == m[x].region.owner )
   && (forall x <- m.Keys, oo <- x.AMFO :: m[oo] in m[x].AMFO)
-//  && forall x <- m.Keys :: (not(inside(x,o)) ==> (m[x] == x))x
+//  && forall x <- m.Keys :: (not(inside(x,o)) ==> (m[x] == x))
 
   && (forall x <- m.Keys |  x.region.Heap? :: x.extra <= x.AMFO)
   && (forall x <- m.Keys |  x.region.Heap? :: x.extra <= m.Keys)
@@ -29,6 +29,100 @@ predicate MapOK(m : Mapping)
   && (forall x <- m.Keys, xo <- x.extra :: m[xo] in m[x].extra)  
 }
 
+
+function MapKV(m : Mapping,   x : Object,  v : Object) : (r : Mapping) 
+  requires MapOK(m)
+  ensures  MapOK(r)
+requires  //the below should be a predicate (from MapKV)
+  && x !in m.Keys
+  //&& COK(x,m.Keys)
+  && x.Ready() && v.Ready()
+  && (forall oo <- (x.AMFO - {x}) :: oo in m.Keys)
+  && (x.region.Heap? == v.region.Heap?)
+  && (x.region.Heap? ==> x.region.owner in x.AMFO)
+  && (x.region.Heap? ==> x.region.owner in m.Keys)
+  && (forall oo <- (x.AMFO - {x}) :: oo in m.Keys &&  m[oo] in v.AMFO)
+  && (x.region.Heap? ==> x.region.owner in (x.AMFO - {x}))
+  && (x.region.Heap? ==> m[x.region.owner] == v.region.owner)
+  && (x.region.Heap? ==> x.extra <= x.AMFO)
+  && (forall xo <- x.extra :: xo in m.Keys)
+  && (forall xo <- x.extra :: m[xo] in v.extra)  
+{
+  reveal COK();
+  var r := m[x:=v];
+//  assert COK(x,m.Keys);
+  assert MapOK(m);
+  assert r.Keys == m.Keys + {x};
+
+  assert m.Keys <= r.Keys;
+  assert forall k <- m.Keys :: k in r.Keys;
+  assert forall k <- r.Keys :: (k in m.Keys) || (k == x);
+  assert forall k <- r.Keys :: 
+    if (k in m.Keys) then r[k] == m[k] else r[k] == v;
+// 
+//   assert (forall x <- r.Keys, oo <- x.AMFO :: r[oo] in r[x].AMFO) by {
+//             assert (forall oo <- x.AMFO :: r[oo] in r[x].AMFO);
+//             assert (forall x <- m.Keys, oo <- x.AMFO :: r[oo] in r[x].AMFO);
+//             assert r.Keys == m.Keys + {x};
+//             assert (forall x <- r.Keys, oo <- x.AMFO :: r[oo] in r[x].AMFO);  
+//             } 
+//   assert (forall x <- r.Keys | x.region.Heap? :: r[x.region.owner] == r[x].region.owner) by {
+//             assert (forall x <- m.Keys | x.region.Heap? :: m[x.region.owner] == r[x].region.owner);
+//             assert (forall x <- m.Keys |  x.region.Heap? :: m[x.region.owner] == r[x].region.owner);
+//             assert r.Keys == m.Keys + {x};
+//             assert (forall x <- r.Keys | x.region.Heap? :: r[x.region.owner] == r[x].region.owner);          
+//             }
+
+  assert (forall x <- r.Keys :: x.region.Heap? == r[x].region.Heap?) by {
+      assert (forall x <- m.Keys :: x.region.Heap? == r[x].region.Heap?); 
+      assert r.Keys == m.Keys + {x};
+      assert (forall x <- r.Keys :: x.region.Heap? == r[x].region.Heap?); 
+  }
+
+   assert (&& (forall x <- m.Keys, xo <- x.extra :: xo in m.Keys)
+           && (forall x <- r.Keys, xo <- x.extra :: r[xo] in r[x].extra)) by {
+      assert (forall x <- m.Keys, xo <- x.extra :: m[xo] in m[x].extra);
+      assert forall k <- r.Keys :: 
+        if (k in m.Keys) then r[k] == m[k] else r[k] == v;      
+      assert (forall x <- m.Keys, xo <- x.extra :: r[xo] in m[x].extra);
+      assert r.Keys == m.Keys + {x};
+      assert x in r.Keys;
+      assert (forall xo <- x.extra :: m[xo] in v.extra);
+      assert (forall x <- r.Keys, xo <- x.extra :: r[xo] in r[x].extra);
+  }  
+
+
+
+  assert (forall x <- r.Keys |  x.region.Heap? :: r[x.region.owner] == r[x].region.owner ) 
+    by {
+      assert MapOK(m);
+      assert (forall x <- m.Keys |  x.region.Heap? ::  m[x.region.owner] == m[x].region.owner );
+      assert forall k <- r.Keys :: 
+        if (k in m.Keys) then r[k] == m[k] else r[k] == v;
+      assert (forall x <- m.Keys |  x.region.Heap? ::  r[x.region.owner] == r[x].region.owner );
+      assert x.region.Heap? ==>  (r[x.region.owner] == r[x].region.owner);
+      assert (forall x <- r.Keys |  x.region.Heap? :: r[x.region.owner] == r[x].region.owner );
+    } 
+
+  assert (forall x <- r.Keys, oo <- x.AMFO :: r[oo] in r[x].AMFO)
+    by {
+      assert MapOK(m);
+      assert (forall x <- m.Keys, oo <- x.AMFO :: m[oo] in m[x].AMFO);
+      assert forall k <- r.Keys :: 
+        if (k in m.Keys) then r[k] == m[k] else r[k] == v;
+      assert (forall x <- m.Keys, oo <- x.AMFO :: r[oo] in r[x].AMFO);
+      assert (forall oo <- x.AMFO - {x} :: r[oo] in v.AMFO);
+      assert r[x] == v;
+      assert (x in x.AMFO) && (v in v.AMFO) && (r[x] in r[x].AMFO);
+      assert (forall x <- r.Keys, oo <- x.AMFO :: r[oo] in r[x].AMFO);
+    } 
+
+
+
+
+  assert MapOK(r);
+  r
+}
 
 
 datatype Map = Map(
@@ -44,6 +138,35 @@ datatype Map = Map(
 
 
 
+   predicate from(other : Map) 
+   // should this be unique or not?
+   // m.from(other) assuming other.MapOK, then I',m Map(OK) and a a "strict but improper extension"
+   // strict - thijngs like oHeap can't change
+   // improper - could be exactly the same as other 
+   //
+   // if most things are OK,  given xown, xm := foo(own, m);
+   // then we should have xm.from(m);  I THINK??
+   //
+  /// what's really annoy6ing is: should I keep track of the first from?
+  // cos usually that's what I need to prove.
+    reads oHeap`fields, oHeap`fieldModes
+    reads ns`fields, ns`fieldModes
+    reads other.oHeap`fields, other.oHeap`fieldModes
+    reads other.ns`fields, other.ns`fieldModes
+
+    requires calid()
+    requires other.calid()
+    {  
+       reveal calid(), calidObjects(), calidOK(), calidMap(), calidSheep();
+       && calid()         //should these be requirements?  
+       && other.calid()   //currently YES because the underlyign thing will require calid and reutnr calid
+       && mapGEQ(m, other.m)
+       && ks    >= other.ks
+       && vs    >= other.vs
+       && o     == other.o
+       && oHeap == other.oHeap
+       && ns    >= other.ns   
+    }
 
     opaque function at(k : Object) : (v : Object)
       //return value corresponding to key k
@@ -98,19 +221,23 @@ datatype Map = Map(
       reads oHeap`fields, oHeap`fieldModes
       reads ns`fields, ns`fieldModes,  v`fields, v`fieldModes     
       requires calid()
+      requires k  in oHeap
       requires k !in ks
-      requires k in oHeap
+      requires k !in m.Keys
+      requires v !in oHeap
+      requires v !in ns
+      requires v !in vs
+      requires v !in m.Values
       requires COK(k, oHeap)
       requires COK(v, oHeap+ns+{v})
       requires ks <= oHeap
       requires k.owners() <= ks  //need to update - all my owners EXCEPT ME!
       requires k.owners() <= m.Keys 
       requires v.owners() <= oHeap+ns //need to hae proceessed all owners first
-      requires v !in vs
-      requires v !in (oHeap + ns)
+      // requires v in (oHeap + ns) // should be a SEPERATIJG COJUNCTION (Below)
+      // requires ((v in oHeap) != (v in ns))  //NOPE for now put it in ns
       requires k.region.Heap? == v.region.Heap?
       requires k.region.Heap? ==> v.region.Heap? && (k.region.owner in m.Keys) && (m[k.region.owner] == v.region.owner)
-      requires k.owners() <= m.Keys
       requires forall ko <- k.owners() :: ko in m.Keys
       requires forall ko <- k.owners() :: m[ko] in v.AMFO
 
@@ -123,13 +250,24 @@ datatype Map = Map(
       requires v.fieldModes == k.fieldModes
 
       ensures  r == Map(m[k:=v], ks+{k}, vs+{v}, o, oHeap, ns+{v})
+      ensures  r.m.Keys == r.ks
+      ensures  r.m.Values == r.vs
       ensures  v in r.ns
       ensures  k in r.ks && r.m[k] == v
       ensures  COK(v, r.oHeap+r.ns)
+      ensures  k in r.m.Keys
+      ensures  v in r.m.Values
+      ensures  r.m == m[k:=v]
+      ensures  r.m == MappingPlusOneKeyValue(this.m,k,v)
+      ensures  mapLEQ(m, r.m)
       ensures  r.calid()
+      ensures  r.from(this)
       {   
         reveal calid(); assert calid();
         var rv := Map(m[k:=v], ks+{k}, vs+{v}, o, oHeap, ns+{v});
+
+
+        assert oXn: oHeap !! ns by { assert calid(); assert calidObjects(); reveal calidObjects();}
 
           assert COK(v, rv.oHeap+rv.ns) by {
             assert COK(v, oHeap+ns+{v});  // from reqs
@@ -146,7 +284,8 @@ datatype Map = Map(
             assert rv.vs == rv.m.Values;
             assert rv.o in rv.oHeap;
             assert rv.ks <= rv.oHeap;
-            assert rv.ns !! rv.oHeap;
+            assert    ns !!    oHeap by { reveal oXn; } 
+            assert rv.ns !! rv.oHeap by { assert rv.oHeap == oHeap; assert rv.ns == ns+{v}; }
             assert rv.vs <= rv.ns + oHeap;
 
             assert rv.calidObjects(); 
@@ -257,19 +396,7 @@ datatype Map = Map(
             }  //MAapOK
 
 
-            assert (forall x <- rv.m.Keys :: (not(inside(x,rv.o)) ==> (rv.m[x] == x))) by 
-            {
-                  reveal rv.calidObjects();
-                  assert ks == m.Keys;
-                  assert rv.ks == rv.m.Keys;
-                  assert (forall x <- ks  :: (not(inside(x,o)) ==> (m[x] == x)));
-                  assert (forall x <- ks  :: (not(inside(x,o)) ==> (rv.m[x] == x)));
-                  assert rv.m[k] == v;
-                  assert (forall x <- {k} :: (not(inside(x,o)) ==> (rv.m[x] == x)));
-                  assert (forall x <- ks+{k} :: (not(inside(x,o)) ==> (rv.m[x] == x)));
-                  assert rv.ks == ks+{k};
-                  assert (forall x <- rv.ks :: (not(inside(x,rv.o)) ==> (rv.m[x] == x)));
-            }
+        
             reveal rv.calidObjects();
             assert ks == m.Keys;
             assert rv.ks == rv.m.Keys;
@@ -317,166 +444,155 @@ datatype Map = Map(
 
 
 
-    opaque function {:isolate_assertions} putOutside(k : Object) : (r : Map)
+    opaque function {:isolate_assertions} {:timeLimit 40} putOutside(k : Object) : (r : Map)
       //put k -> k into map, k oustide o
       reads oHeap`fields, oHeap`fieldModes
       reads ns`fields, ns`fieldModes
       requires calid()
       requires k !in ks
       requires k !in vs
+      requires k !in m.Keys
+      requires k !in m.Values
       requires k in oHeap
       requires COK(k, oHeap)
-      requires k.owners() <= ks   //need to update - all my owners EXCEPT ME!
+      requires k.owners() <= ks
       requires not(inside(k, o))
+
+requires
+  && k !in m.Keys
+  && COK(k,oHeap)
+  && k.Ready()
+  && k.AllOwnersAreWithinThisHeap(ks)
+  && (forall oo <- k.AMFO - {k}:: oo in m.Keys)
+  //  && (k.region.Heap? ==> m[k].region.Heap?)  WHATR THE FUCK k at in the map!
+  && (k.region.Heap? ==> k.region.owner in k.AMFO)
+  && (k.region.Heap? ==> k.region.owner in m.Keys)
+  // && (k.region.Heap? ==> m[k.region.owner] == m[k].region.owner )
+  //  && (forall oo <- k.AMFO :: m[oo] in m[k].AMFO)
+  && (k.region.Heap? ==> k.extra <= k.AMFO)
+  && (forall xo <- k.extra :: xo in m.Keys)
+  // && (forall xo <- k.extra :: m[xo] in m[k].extra) 
+
+
+
+
+      requires forall kx <- k.extra :: kx in m.Keys
+      requires forall kx <- k.extra :: m[kx] == kx
 
       ensures r == Map(m[k:=k], ks+{k}, vs+{k}, o, oHeap, ns)
       ensures k in r.ks && r.m[k] == k
-      ensures k !in this.m.Keys
-      ensures k !in this.m.Values
-      ensures r.m == MappingPlusOneKeyValue(this.m,k,k)
+      ensures k in r.m.Keys
+      ensures k in r.m.Values
+      ensures MapOK(r.m)
+      ensures weirdo() && (r.m == MapKV(this.m,k,k))
       ensures mapLEQ(m, r.m)
       ensures r.calid()
-      { 
-      reveal calid(); assert calid();
-      var rv := Map(m[k:=k], ks+{k}, vs+{k}, o, oHeap, ns);
+      ensures r.from(this)
+{
 
-          assert rv.calidObjects() by {
-            reveal rv.calidObjects();
+assert  //the below should be a predicate (from MapKV)
+  && k !in m.Keys
+  //&& COK(k,m.Keys)
+  && (forall oo <- k.AMFO - {k} :: oo in m.Keys)
+  //&& (k.region.Heap? ==> m[k].region.Heap?)
+  && (k.region.Heap? ==> k.region.owner in k.AMFO)
+  && (k.region.Heap? ==> k.region.owner in m.Keys)
+  //&& (k.region.Heap? ==> m[k.region.owner] == m[k].region.owner )
+  //&& (forall oo <- k.AMFO :: m[oo] in m[k].AMFO)
+  && (k.region.Heap? ==> k.extra <= k.AMFO)
+  && (forall xo <- k.extra :: xo in m.Keys)
+  //&& (forall xo <- k.extra :: m[xo] in m[k].extra) 
+  ;
 
-            assert rv.ks == rv.m.Keys;
-            assert rv.vs == rv.m.Values;
-            assert rv.o in rv.oHeap;
-            assert rv.ks <= rv.oHeap;
-            assert rv.ns !! rv.oHeap;
-            assert rv.vs <= rv.ns + oHeap;
+  reveal calid();
+  assert calid();
+  reveal calidObjects();
+  assert calidObjects();
+  reveal calidOK();
+  assert calidOK();
+  
+  assert ks == m.Keys;
+  assert calidMap();
+  reveal calidMap();
+  assert calidSheep();
+  reveal calidSheep();
 
-            assert rv.calidObjects(); 
-          }
+  assert MapOK(m);
+  assert CallOK(oHeap);
 
-          assert k !in vs; // from reqs
-            assert vs == m.Values by { 
-            assert calid();
-            reveal calid();
-            assert calidObjects();
-            reveal calidObjects();
-            assert vs == m.Values;
-                   }
-          assert k !in m.Values;
+  var numap := MapKV(m,k,k);
+  assert MapOK(numap);
 
+  var rv := Map(numap, ks+{k}, vs+{k}, o, oHeap, ns);
 
-          assert rv.calidOK() by {
-            reveal rv.calidOK();
-            assert COK(rv.o, rv.oHeap);
-            assert CallOK(rv.oHeap);
-            CallOKfromCOK(k, oHeap);
-            assert rv.ks <= rv.oHeap by {
-                assert calidObjects();
-                reveal calidObjects();
-            }
-            assert CallOK(ks, oHeap);
-            CallOKtoSubset(ks, oHeap);
-            CallOKWiderFocus(ks, {k}, oHeap);
-            assert CallOK(rv.ks, rv.oHeap);
-            CallOKWiderContext({k}, oHeap, ns);
-            CallOKtoSubset(vs, oHeap+ns);
-            CallOKWiderFocus(vs, {k}, oHeap+ns);
-            assert CallOK(rv.vs, rv.oHeap+ns);
-            assert CallOK(rv.ns, rv.oHeap+ns);
-            reveal rv.calidOK(); assert rv.calidOK();
-          }
+  assert rv == Map(m[k:=k], ks+{k}, vs+{k}, o, oHeap, ns);
+  assert k in rv.ks && rv.m[k] == k;
+  assert k in rv.m.Keys;
+  assert k in rv.m.Values;
+  assert MapOK(rv.m);
+  assert weirdo() && (rv.m == MapKV(this.m,k,k));
+  assert mapLEQ(m, rv.m);
+  assert rv.calidObjects();
+  
 
-            reveal rv.calidMap();
-            assert MapOK(rv.m) by {
-                assert MapOK(m);
-                assert COK(k, oHeap);
-                reveal COK();
-                assert rv.ks == ks + {k};          
-                assert rv.m.Keys == m.Keys + {k};
+  assert rv.calidOK() by {
+      assert (rv.o in rv.oHeap);
+      assert (rv.ks <= rv.oHeap);
+      assert (rv.vs <= rv.oHeap+ns);
+      assert COK(rv.o, rv.oHeap) by { assert COK(o,oHeap);  assert rv.oHeap == oHeap; assert rv.o == o; }
+      assert CallOK(rv.oHeap)    by { assert CallOK(oHeap); assert rv.oHeap == oHeap; }
+      assert CallOK(rv.ks, rv.oHeap) by { assert CallOK(ks, oHeap); 
+                                          assert COK(k,oHeap); 
+                                          CallOKfromCOK(k,oHeap);
+                                          CallOKWiderFocus(ks,{k},oHeap);
+                                          assert rv.oHeap == oHeap; 
+                                          assert rv.ks == ks+{k}; }
+      assert CallOK(rv.vs, rv.oHeap+rv.ns) by { assert CallOK(vs, oHeap+ns);
+                                                assert COK(k,oHeap);
+                                                CallOKfromCOK(k,oHeap);
+                                                CallOKWiderContext({k},oHeap,ns);
+                                                CallOKWiderFocus(vs,{k},oHeap+ns); 
+                                                assert rv.oHeap+rv.ns == oHeap+ns;
+                                                assert rv.vs == vs+{k}; }
+      assert CallOK(rv.ns, rv.oHeap+rv.ns) by { assert CallOK(ns, oHeap+ns);
+                                                assert rv.oHeap == oHeap;
+                                                assert rv.ns == ns; } 
+      assert rv.calidOK();
+  } 
 
-                reveal rv.calidObjects();
-                assert rv.calidObjects();
-                reveal calidObjects();
-                assert calidObjects();
+  reveal rv.calidMap();
+  assert rv.calidMap();
+  reveal calidObjects(); assert calidObjects();
+  reveal calidOK(); assert calidOK(); 
+  reveal rv.calidSheep();
+  assert rv.ks == rv.m.Keys;
+  reveal AreWeNotMen(); 
+  assert (forall x <- rv.ks :: AreWeNotMen(x, rv));
+  assert (forall x <- rv.ks :: x.fieldModes == rv.m[x].fieldModes);
+  assert rv.calidSheep();
+  reveal rv.calid();
+  assert rv.calid();
+  assert rv.from(this);
 
-                assert rv.m.Keys == rv.ks;
+  rv
+}
 
-                assert forall x <- m.Keys :: x.AMFO <= ks by { 
-                  assert forall x <- m.Keys, oo <- x.AMFO :: oo in m.Keys;
-                }  
-                assert k.owners() <= ks;
-                assert forall x <- m.Keys+{k} :: x.owners() <= ks;
-                assert forall x <- m.Keys+{k} :: x.owners() <= ks+{k};
-                assert (ks+{k}) == m.Keys+{k} == rv.ks == rv.m.Keys;
-                assert forall x <- rv.m.Keys :: x.AMFO <= rv.m.Keys;
-                assert forall x <- rv.m.Keys, oo <- x.AMFO :: oo in rv.m.Keys;
-
-                assert (forall x <- rv.m.Keys :: x.region.Heap? == rv.m[x].region.Heap?);
-                assert (forall x <- rv.m.Keys |  x.region.Heap? :: x.region.owner in x.AMFO);
-                assert (forall x <- rv.m.Keys |  x.region.Heap? :: x.region.owner in rv.m.Keys);
-                assert (forall x <- rv.m.Keys |  x.region.Heap? :: rv.m[x.region.owner] == rv.m[x].region.owner );
-
-                assert MapOK(rv.m);
-            } 
-
-            assert (forall x <- rv.m.Keys :: (not(inside(x,rv.o)) ==> (rv.m[x] == x))) by 
-            {
-                  reveal rv.calidObjects();
-                  assert ks == m.Keys;
-                  assert rv.ks == rv.m.Keys;
-                  assert (forall x <- ks  :: (not(inside(x,o)) ==> (m[x] == x)));
-                  assert (forall x <- ks  :: (not(inside(x,o)) ==> (rv.m[x] == x)));
-                  assert rv.m[k] == k;
-                  assert (forall x <- {k} :: (not(inside(x,o)) ==> (rv.m[x] == x)));
-                  assert (forall x <- ks+{k} :: (not(inside(x,o)) ==> (rv.m[x] == x)));
-                  assert rv.ks == ks+{k};
-                  assert (forall x <- rv.ks :: (not(inside(x,rv.o)) ==> (rv.m[x] == x)));
-            }
-            reveal rv.calidObjects();
-            assert ks == m.Keys;
-            assert rv.ks == rv.m.Keys;
-            assert (forall x <- rv.ks :: (not(inside(x,rv.o)) ==> (rv.m[x] == x)));
-            assert (forall x <- rv.m.Keys, oo <- x.AMFO :: rv.m[oo] in rv.m[x].AMFO);
-            assert (forall x <- ks, oo <- x.AMFO :: m[oo] in m[x].AMFO);
-            reveal rv.calidMap();
-            assert rv.calidMap();
-          
-            reveal rv.calidSheep();
-                reveal rv.calidObjects();
-                assert ks == m.Keys;
-                assert rv.ks == rv.m.Keys;
-            assert not(inside(k, o));
-            reveal calidMap();
-            assert calidMap();
-            reveal calidSheep();
-            assert calidSheep();
-
-          assert forall x <- ks :: AreWeNotMen(x, this);
-
-          assert rv.ks == rv.m.Keys == (ks+{k});
-
-
-          assert calidSheep();
-          reveal rv.calidSheep();
-          //reveal UniqueMapEntry();
-
-          assert ks == m.Keys;
-
-          reveal AreWeNotMen();  
-          reveal UniqueMapEntry();
-          assert forall x <- ks  :: AreWeNotMen(x, this);
-          assert forall x <- {k} :: AreWeNotMen(x, rv);
-          assert forall x <- rv.m.Keys :: AreWeNotMen(x, rv);
-          
-
-
-          assert rv.calidSheep();
-
-          reveal rv.calid(); assert rv.calid();
-
-          rv
-        
-   }
-
+predicate weirdo() 
+ requires calid()
+ ensures  MapOK(m)
+ reads oHeap`fields, oHeap`fieldModes
+ reads ns`fields, ns`fieldModes
+ {
+      reveal calid();
+      assert calid();
+      reveal calidObjects();
+      assert calidObjects();
+      assert ks == m.Keys;
+      reveal calidMap();
+      assert calidMap();
+      assert MapOK(m);
+  MapOK(m)
+ }
 
 
 
@@ -485,10 +601,90 @@ opaque predicate {:onlyNUKE} AreWeNotMen(x : Object,  rv : Map)  //hmmm wgt etc?
       reads ns`fields, ns`fieldModes
       requires x in rv.m.Keys
    {
-      &&      ((inside(x,rv.o)) ==> (rv.m[x] in rv.ns))
+      && ((   (inside(x,rv.o))) ==> rv.m[x] in rv.ns)
      // &&     (inside(x,rv.o)) ==> (UniqueMapEntry(rv.m,x))
       && ((not(inside(x,rv.o))) ==> (rv.m[x] == x)) 
    }
+
+lemma WeAreDevo()
+  requires calid()
+  ensures  forall k <- m.Keys :: AreWeNotMen(k,this)
+  {
+            reveal calid();
+            assert calid();
+            reveal calidOK();
+            assert calidOK();
+            reveal calidObjects();
+            assert calidObjects();
+            reveal calidMap();
+            assert calidMap();
+            reveal calidSheep();
+            assert calidSheep();
+
+            assert  forall k <- m.Keys :: AreWeNotMen(k,this);
+  }
+
+
+static lemma AintNoSunshine(x : Object, rv : Map)
+//
+    requires not(inside(x,rv.o))
+    requires x !in rv.m.Keys
+
+    requires rv.calid()
+    requires forall k <- rv.m.Keys :: rv.AreWeNotMen(k,rv)
+    requires x  in rv.oHeap
+    requires x !in rv.ns
+
+    ensures  x !in rv.m.Values
+{
+    assert rv.calid();
+
+    reveal rv.calid();
+    assert rv.calid();
+    reveal AreWeNotMen();
+    assert forall k <- rv.m.Keys :: rv.AreWeNotMen(k,rv);
+
+    reveal rv.calidObjects();
+    assert rv.calidObjects();  
+    reveal rv.calidOK();
+    assert rv.calidOK();
+    reveal rv.calidOK();
+    assert rv.calidOK();
+    reveal rv.calidSheep();
+    assert rv.calidSheep();
+
+
+    forall k <- rv.m.Keys 
+      ensures (x !in rv.m.Values)
+      {
+        if (inside(k,rv.o)) 
+          { assert rv.AreWeNotMen(k, rv);
+            assert (rv.m[k] in rv.ns);
+            assert  x !in rv.ns;
+            assert (rv.m[k] != x);
+          } 
+        else if (k != x)
+          { 
+            assert not(inside(k,rv.o));
+            assert rv.AreWeNotMen(k, rv);
+            assert (rv.m[k] == k);
+            assert  rv.m[k] != x;
+          } 
+        else
+          {
+            assert k in rv.m.Keys;
+            assert {:contradiction} k == x;
+            assert {:contradiction} not(inside(k,rv.o));
+            assert {:contradiction} rv.AreWeNotMen(k, rv);
+            assert {:contradiction} rv.m[k] == k;
+            assert {:contradiction} rv.m[k] == x; 
+            assert {:contradiction} rv.m[x] == x;    
+            assert {:contradiction} x in rv.m.Values;
+            assert {:contradiction} x in rv.m.Keys;
+            assert {:contradiction} false; 
+          }
+      }
+}                                           
 
 
 
@@ -648,6 +844,16 @@ lemma SubsetOfKeysOfExtendedMap(subset : set<Object>, left : Map, right : Map)
   }
 
 
+lemma Yowl(k : Object, kk : set<Object>)
+  requires forall kx <- k.extra :: kx in kk
+  ensures  k.extra <= kk
+{}
+
+
+lemma Howl(k : Object, kk : set<Object>)
+  requires k.extra <= kk
+  ensures  forall kx <- k.extra :: kx in kk
+{}
 
 
 
@@ -658,7 +864,7 @@ lemma SubsetOfKeysOfExtendedMap(subset : set<Object>, left : Map, right : Map)
 //actual cloning methods
 
 
-method {:onlyCVM}  Clone_Via_Map(a : Object, m' : Map)
+method {:onlyCVM}   Clone_Via_Map(a : Object, m' : Map)
     returns (b : Object, m : Map)
 //entry point for Clone - clones a according to map m'
 //call with m' empty    
@@ -667,6 +873,8 @@ method {:onlyCVM}  Clone_Via_Map(a : Object, m' : Map)
   requires m'.calid()
   requires a in m'.oHeap  //technically redundant given COKx
   requires COK(a, m'.oHeap)
+
+  requires a.extra == {} //extra not yet cloned
 
   //ensures  (m.oHeap - m.ks) < (m'.oHeap - m'.ks) 
 
@@ -686,13 +894,19 @@ method {:onlyCVM}  Clone_Via_Map(a : Object, m' : Map)
   ensures  mapLEQ(m'.m,m.m)
   ensures  m.ks >= m'.ks + {a}
   ensures  m.vs >= m'.vs + {b}
+  ensures  m.from(m')
 
   ensures  m.o == m'.o
   ensures  m.oHeap == m'.oHeap
   ensures  m.ns >= m'.ns
 //  ensures  if (inside(a, m'.o)) then (b in m.ns) else (b == a)
 //  ensures  reveal m.calid(); reveal m.calidMap(); assert m.calid(); assert 
-  ensures MapOK(m.m) && a.AMFO <= m.ks
+  ensures MapOK(m.m) 
+  ensures a.AMFO <= m.ks  //seems weird but we are populating m, right...
+  ensures a.extra <= m.ks //ditto?
+
+  //ensures b.AMFO == set x <- a.AMFO :: m.m[x]
+
 
   ensures  unchanged(a)
   ensures  unchanged(m'.oHeap+m'.ns)
@@ -767,7 +981,7 @@ modifies {} // only modifes objecst allocated aftrer this point?
 
 
 
-        assert  MapOK(m.m) && (a.AMFO <= m.ks) by
+        assert MapOK(m.m) && (a.AMFO <= m.ks) && (a.extra <= m.ks)  by
           {
             reveal m.calid();
             assert m.calid();
@@ -777,7 +991,10 @@ modifies {} // only modifes objecst allocated aftrer this point?
             assert m.calidObjects();
             reveal m.calidMap();
             assert m.calidMap();
-            assert  MapOK(m.m) && a.AMFO <= m.ks;
+            assert m.ks == m.m.Keys;
+            assert MapOK(m.m) && a.AMFO <= m.m.Keys;
+            assert MapOK(m.m) && a.AMFO <= m.ks;
+            assert a.extra <= m.ks;
           }
 
             reveal m.calid();
@@ -789,14 +1006,16 @@ modifies {} // only modifes objecst allocated aftrer this point?
   assert  m.o     == m'.o;
   assert  m.oHeap == m'.oHeap;
   assert  m.ns    >= m'.ns;
-
+//  reveal  m.from();
       return;
   } // a in ks, already cloned
 
   assert unchanged(a) && unchanged(m.oHeap);
 
-  assert a !in m.ks; 
-  assert a !in m'.ks; 
+  assert a !in m.ks;
+  assert a !in m'.ks;
+  // assert a !in m.vs;
+  // assert a !in m'.vs; 
 
 ///case analysis...
   if (outside(a,m.o)) {
@@ -805,7 +1024,39 @@ modifies {} // only modifes objecst allocated aftrer this point?
       if (a.region.Heap?) {
         print "Clone_Via_Map outside owners:", fmtobj(a), " owned by ", fmtobj(a.region.owner) ,"\n";
 
-        b, m := Clone_Outside_Heap(a, m);
+        assert 
+          && (a !in m.m.Keys)
+          && (a !in m.ns) 
+          && (m.m.Values == m.vs)
+          by {
+            reveal m.calid();
+            assert m.calid();
+            reveal m.calidOK();
+            assert m.calidOK();
+            reveal m.calidObjects();
+            assert m.calidObjects();
+            reveal m.calidMap();
+            assert m.calidMap();
+            assert m.ks == m.m.Keys;
+            reveal m.calidSheep();
+            assert m.calidSheep();
+            assert a !in m.m.Keys; 
+            assert a in m.oHeap;
+            assert m.oHeap !! m.ns;
+            assert a in m.oHeap;
+            assert m.m.Values == m.vs;
+        }
+
+        m.WeAreDevo();
+        Map.AintNoSunshine(a,m);
+
+        assert a !in m.vs by {
+            assert a !in m.m.Values;
+            assert m.m.Values == m.vs;
+            assert a !in m.vs;
+        }
+          b, m := Clone_Outside_Heap(a, m);
+
 
       //END outside  HEAP OBJECT
     } 
@@ -831,8 +1082,10 @@ modifies {} // only modifes objecst allocated aftrer this point?
   assert m.calidSheep();
 
   assert a in m.ks;
-  assert  b.fieldModes == a.fieldModes;
+  assert b.fieldModes == a.fieldModes;
 
+      assert forall kx <- a.extra :: m.m[kx] in m.m[a].extra;
+      assert a.extra <= m.ks;
 
   return;  //we may as well just return here.
            //we've done all we need to do.  I think.
@@ -884,9 +1137,6 @@ modifies {} // only modifes objecst allocated aftrer this point?
   //assert b !in m'.ns;
 
 
-  assert  m.o     == m'.o;
-  assert  m.oHeap == m'.oHeap;
-  assert  m.ns    >= m'.ns;
 //  assert  b.fields.Keys == {};
 
   assert  b.fieldModes.Keys == a.fieldModes.Keys;
@@ -896,7 +1146,14 @@ modifies {} // only modifes objecst allocated aftrer this point?
 
   assert  b.fieldModes == a.fieldModes;
 
-
+//  assert m.from(m') by {
+//      reveal m.from();
+      assert  m.o     == m'.o;
+      assert  m.oHeap == m'.oHeap;
+      assert  m.ns    >= m'.ns;
+    
+      assert m.from(m');
+//  }
 }
 
 
@@ -963,8 +1220,7 @@ method  {:onlyCFM} Clone_All_Fields(a : Object, b : Object, m' : Map)
   ensures  CallOK(m.oHeap)
   ensures  COK(a, m.oHeap)
   ensures  COK(b, m.oHeap+m.ns)
-  //  ensures  CallOK(m.oHeap
-    ensures  CallOK(m.vs, m.oHeap+m.ns)
+  ensures  CallOK(m.vs, m.oHeap+m.ns)
   ensures  CallOK(m.ns, m.oHeap+m.ns)
 
   ensures  m.o     == m'.o
@@ -1014,7 +1270,6 @@ print "<<<<<<<<<<<\n";
 
 
 //assert fresh(b);
-// assume fresh(b);          
 assert  b.fields.Keys == {}; 
 assert b in m.vs;
 
@@ -1312,6 +1567,7 @@ assert m.calidObjects();
   
     return;
 }//end Clone_All_Fields
+ 
 
 
 
@@ -1320,10 +1576,12 @@ method {:isolate_assertions} {:timeLimit 40} Clone_Outside_Heap(a : Object, m' :
       returns (b : Object, m : Map)
   decreases (m'.oHeap - m'.ks), a.AMFO, (a.fields.Keys), 15 //Clone_Outside_Heap
 
-
+  requires a.extra == {} //extra not yet cloned
 
 //this case
   requires a !in m'.ks
+  requires a !in m'.vs
+
   requires outside(a,m'.o)
   requires a.region.Heap?
 
@@ -1331,7 +1589,7 @@ method {:isolate_assertions} {:timeLimit 40} Clone_Outside_Heap(a : Object, m' :
   requires m'.calid()
   requires a in m'.oHeap 
   requires COK(a, m'.oHeap)
-
+  
   ensures  m.calid()
   ensures  a == b
   ensures  a in m.ks
@@ -1350,7 +1608,11 @@ method {:isolate_assertions} {:timeLimit 40} Clone_Outside_Heap(a : Object, m' :
   ensures  m.ns >= m'.ns
 //  ensures  if (inside(a, m'.o)) then (b in m.ns) else (b == a)
 //  ensures  reveal m.calid(); reveal m.calidMap(); assert m.calid(); assert 
-  ensures MapOK(m.m) && a.AMFO <= m.ks
+  ensures MapOK(m.m) 
+  ensures a.AMFO <= m.ks  //seems weird but we are populating m, right...
+  ensures a.extra <= m.ks //ditto?
+
+  //ensures b.AMFO == set x <- a.AMFO :: m.m[x] 
 
   ensures b.fieldModes == a.fieldModes
 //  ensures b.fields.Keys == a.fields.Keys
@@ -1359,6 +1621,14 @@ method {:isolate_assertions} {:timeLimit 40} Clone_Outside_Heap(a : Object, m' :
   modifies {}
   {
         m := m';
+        assert m.ks == m'.ks;
+        assert a !in m.ks;
+        assert a !in m.vs;
+
+        assert m == m';
+        assert m.m == m'.m;
+        assert mapLEQ(m'.m,m.m);
+        assert m.from(m');
 
         print "Clone_Outside_Heap outside owners:", fmtobj(a), " owned by ", fmtobj(a.region.owner) ,"\n";
 print "VARIANT COH ", |(m'.oHeap - m'.ks)|, " ", |a.AMFO|, " ", |(a.fields.Keys)|, " ", 15, "\n";
@@ -1402,16 +1672,48 @@ print "VARIANT COH ", |(m'.oHeap - m'.ks)|, " ", |a.AMFO|, " ", |(a.fields.Keys)
             assert COK(a.region.owner, m.oHeap); 
           }
 
+    assert CallOK(a.extra, m.oHeap) by {
+      assert a.OwnersValid();
+            assert a.extra <= a.AMFO;
+            assert CallOK(m.oHeap);
+            assert COK(a,m.oHeap);
+            assert a.extra <= m.oHeap by {
+                assert COK(a,m.oHeap);
+                reveal COK();
+                assert a.extra <= m.oHeap;
+            }
+            CallOKNarrowFocus(a.extra, m.oHeap);
+            reveal CallOK();
+            assert COK(a, m.oHeap);
+            a.CallMyOwnersWillWitherAway(a, m.oHeap);
+            assert CallOK(a.extra, m.oHeap); 
+    }
+
+
 //preconditions for the call..
   // assert m.calid();
   // assert a.region.owner in m.oHeap;  
 assert COK(a.region.owner, m.oHeap); 
   // assert outside(a.region.owner, m.o); //TEMP TO WRITEOUTSIDE CASE
 
+reveal COK(); assert a.extra == {}; //extra not yet cloned
+
         var rowner, rm := Clone_Via_Map(a.region.owner, m);
-
-assert MapOK(rm.m) && rowner.AMFO <= rm.ks;
-
+        assert a.region.owner in rm.ks;
+        assert a.region.owner.AMFO <= rm.ks;
+        assert a.AMFO == a.region.owner.AMFO + a.extra + {a};
+        assert rm.from(m);
+        assert rm.from(m');
+assert MapOK(rm.m); 
+reveal rm.calid(); assert rm.calid();
+reveal rm.calidObjects(); assert rm.calidObjects();
+        assert rm.ks == rm.m.Keys;
+reveal rm.calidMap(); assert  rm.calidMap(); 
+        assert (forall x <- rm.m.Keys, oo <- x.AMFO :: rm.m[oo] in rm.m[x].AMFO);
+        assert (forall x <- rm.ks,     oo <- x.AMFO :: rm.m[oo] in rm.m[x].AMFO);
+        assert rm.ks >= m'.ks;
+        assert mapLEQ(m'.m,rm.m);    
+        assert rm.from(m);
 
 ///WHY THE FuCK DO I NEED TO DO THIS?
 ///BEST GUESS TO EnSURE ALL The OWNERS of a are in the map
@@ -1425,7 +1727,7 @@ assert MapOK(rm.m) && rowner.AMFO <= rm.ks;
       //or won't the recursive call handle it anyway??
         if (a in rm.ks) {
             m := rm;
-
+            assert m.from(rm);  
             reveal m.calid();
             assert m.calid();  
             reveal m.calidObjects();
@@ -1459,64 +1761,327 @@ assert MapOK(rm.m) && rowner.AMFO <= rm.ks;
             assert COK(b, m.oHeap+m.ns);
 
             assert b.fieldModes == a.fieldModes;
-
+            assert m.from(m');
             return; //should work because Clone_Via_Map meets all the conditiosn, right???
-        }
+        }  //end if a in rm.ks
  
 
-        assert a !in rm.ks;
+        assert a !in rm.ks; 
+        assert a !in rm.vs by { 
+          
+          
+                assert not(inside(a,rm.o));
+                assert a !in rm.m.Keys;
+                assert rm.calid(); 
+                rm.WeAreDevo();
+                assert forall k <- rm.m.Keys :: rm.AreWeNotMen(k,rm);
+                assert a  in rm.oHeap;
+                assert a !in rm.ns;
+          
+          
+          
+          Map.AintNoSunshine(a, rm);
+          assert a !in rm.vs; }
+        assert rm.ks >= m'.ks;
+        assert mapLEQ(m'.m,rm.m);
+        assert rm.from(m');
 
 //    //maintaing MapOK
-        assert AMFOOKRM: a.owners() <= rm.ks by {
-            reveal rm.calid();
-            assert rm.calid();
-            reveal rm.calidMap();
-            assert rm.calidMap();
-            assert MapOK(rm.m);
-            reveal rm.calidObjects();
-            assert rm.calidObjects();             
-            assert (forall x <- rm.ks, oo <- x.AMFO :: oo in rm.ks);
-            assert a.owners() <= rm.ks;
-        }     
+//         assert AMFOOKRM: a.owners() <= rm.ks by {
+//             reveal rm.calid();
+//             assert rm.calid();
+//             reveal rm.calidMap();
+//             assert rm.calidMap();
+//             assert MapOK(rm.m);
+//             reveal rm.calidObjects();
+//             assert rm.calidObjects();             
+//             assert (forall x <- rm.ks, oo <- x.AMFO :: oo in rm.ks);
+//             assert a.owners() <= rm.ks by {
+//                reveal COK(); 
+//                assert COK(a,m.oHeap); 
+//                assert a.AMFO <= m.oHeap;
+// //               assert a.owners() <= rm.ks;
+//                }
+//         }5
 
 
 
         assert a in rm.oHeap; 
         assert COK(a, rm.oHeap);
         reveal COK();
-        assert a.owners() <= rm.ks;
+        assert a.AMFO <= rm.oHeap;
+      //  assert a.owners() <= rm.ks;
         OutsidersArentMapValues(a,rm);
         assert a !in rm.vs;
         assert a !in rm.ks;
         assert not(inside(a, rm.o)); 
 
         //m := rm[a:=b];     
-        m := rm.putOutside(a);
+
+
+        assert COK(a, rm.oHeap);
+
+        assert rm.calid();
+        assert a in rm.oHeap;
+        assert COK(a, rm.oHeap);
+        assert a.extra <= rm.oHeap; 
+
+        assert CallOK(rm.oHeap) by {
+          reveal rm.calid(), rm.calidOK();
+          assert rm.calid();
+          assert rm.calidOK();
+          reveal CallOK(), COK();
+          assert CallOK(rm.oHeap);
+        }
+
+
+        var xm := rm;
+        assert xm.ks >= m'.ks;
+        assert mapLEQ(m'.m,xm.m);    
+        assert xm.from(rm);
+        assert xm.from(m');
+
+        assert a !in xm.ks;
+        assert a !in xm.vs;
+
+
+        var MX := a.extra - xm.ks;
+        assert MX <= a.extra;
+        var xo : Object;
+        var rr : Object;
+        var oldmks  : set<Object>;  //dont fucking ask
+        var oldmok :=  false;
+
+        assert !oldmok;
+        assert xm == rm;
+        assert xm.ks >= (m'.ks);
+        assert mapLEQ(m'.m,xm.m);    
+        assert xm.from(m');
+
+        assert a !in xm.ks;
+
+        while ((MX != {}) && (a !in xm.ks))
+          decreases MX
+          invariant MX == a.extra - xm.ks
+          invariant MX <= a.extra
+          invariant xm == rm
+          invariant xm.calid()
+          invariant rm.calid()
+          invariant m'.calid()
+          invariant xm.from(m')  
+          invariant MX <= xm.oHeap            
+          invariant CallOK(xm.oHeap)    
+          invariant a.AMFO - {a} <= xm.ks + MX
+          invariant a.extra <= a.AMFO
+          invariant oldmok ==> assigned(oldmks)
+          invariant oldmok ==> (xm.ks > oldmks)
+          invariant m'.oHeap == xm.oHeap
+          invariant oldmok ==> ((m'.oHeap - oldmks) > (xm.oHeap - xm.ks))
+          invariant xm.ks >= (m'.ks)
+          invariant xm.vs >= (m'.vs)
+          invariant a !in xm.ks
+        {
+          assert xm == rm;
+          xo :| xo in MX;
+          assert xo in MX;
+          MX := MX - {xo};
+           
+          assert xm.calid();
+          assert xo in xm.oHeap;
+          COKfromCallOK(xo,xm.oHeap);
+          assert COK(xo,xm.oHeap);
+          assert xo !in xm.ks;
+        
+        
+          assert oldmok ==> (m'.oHeap - oldmks) > (xm.oHeap - xm.ks);
+
+assert xo in a.AMFO;
+assert a.Ready();
+assert xo in a.extra;
+assert a.AMFO > xo.AMFO;
+
+
+          assert (m'.oHeap) == m'.oHeap == xm.oHeap;
+          assert xm.ks >= (m'.ks);
+          assert xm.from(m');
+
+  assert  mapLEQ(m'.m,xm.m) by 
+               { reveal xm.calid(); assert xm.calid();
+                 reveal xm.calidObjects(); assert xm.calidObjects();
+                 assert m'.ks <= xm.ks;
+                 assert m'.vs <= xm.vs; 
+                 assert m'.ks == m'.m.Keys;
+                 assert m'.vs == m'.m.Values;       
+                 assert xm.ks == xm.m.Keys;
+                 assert xm.vs == xm.m.Values;                              
+                 assert m'.m.Keys <= xm.m.Keys;
+                 assert m'.m.Values <= xm.m.Values;
+                 assert forall k <- m'.m.Keys :: k in xm.m.Keys;
+      assert forall k <- m'.m.Keys :: k in xm.m.Keys && (m'.m[k] == xm.m[k]);
+                }
+        
+
+                  assert xm.ks >= m'.ks;
+                assert a !in xm.ks;          
+
+          assert ((m'.oHeap - m'.ks)) >= (xm.oHeap - xm.ks);
+
+assert  ((a.AMFO)
+  decreases to
+        (xo.AMFO));
+      
+        assert ((m'.oHeap - m'.ks), 
+               (a.AMFO),
+               (a.fields.Keys), 
+               (15) 
+          decreases to 
+               xm.oHeap - xm.ks, 
+               xo.AMFO, 
+               xo.fields.Keys, 
+               20);
+
+      
+          rr, rm := Clone_Via_Map(xo, xm);
+          assert rm.ks >= m'.ks;
+          assert mapLEQ(m'.m,rm.m);    
+          assert rm.from(m');
+
+      if (a in rm.ks) { 
+                m := rm;
+                assert m.calidObjects() by {  reveal m.calid(); assert  m.calid();  }
+                assert  a in m.ks by { reveal m.calidObjects(); assert m.calidObjects(); }
+                assert  a in m.m.Keys by { reveal m.calidObjects(); assert m.calidObjects(); }
+                b := m.m[a];
+                //
+
+                assert  b in m.vs by { reveal m.calidObjects(); assert m.calidObjects();  assert b in m.m.Values; }
+                assert  b in m.m.Values by { reveal m.calidObjects(); assert m.calidObjects(); }
+                assert m.calidOK() by {  reveal m.calid(); assert  m.calid();  }
+                assert  a in m.m.Keys && m.at(a) == b; 
+                assert  COK(b, m.oHeap+m.ns) by {
+                assert b in m.vs;
+                assert CallOK(m.vs, m.oHeap+m.ns) by { reveal m.calidOK(); }
+                COKfromCallOK(b, m.vs, m.oHeap+m.ns);   }
+
+                assert m.from(m');
+
+                assert  mapLEQ(m'.m,m.m) by 
+                        { reveal m.calidObjects(); assert m.calidObjects();
+                          assert m'.ks <= m.ks;
+                          assert mapLEQ(m'.m,m.m);    
+                          assert m'.m.Keys <= m.m.Keys;
+                          assert m'.m.Values <= m.m.Values;
+                          }
+                assert  m.ks >= m'.ks + {a} by { reveal m.calidObjects(); assert m.calidObjects(); }
+                assert  m.vs >= m'.vs + {b} by { reveal m.calidObjects(); assert m.calidObjects(); }
+                assert  m.o == m'.o;
+                assert  m.oHeap == m'.oHeap;
+                assert  m.ns >= m'.ns;
+                assert MapOK(m.m);
+                assert forall x <- m.m.Keys, oo <- x.AMFO :: oo in m.m.Keys;
+                assert  a in m.m.Keys;
+                assert forall oo <- a.AMFO :: oo in m.m.Keys;
+                assert a.AMFO <= m.m.Keys;
+                assert m.ks == m.m.Keys by { reveal m.calidObjects(); assert m.calidObjects(); }
+                assert a.AMFO <= m.ks;
+                assert a.extra <= m.ks;
+
+
+            
+                assert  a == b by {
+                      reveal m.calid();
+                      assert m.calidMap();
+                      reveal m.calidMap();
+                  //    assert (forall x <- m.ks :: (not(inside(x,m.o)) ==> (m.m[x] == x)));
+                      assert not(inside(a,m.o));
+                      assert m.m[a] == a;
+                      assert a == b;
+                  }
+
+             assert (b.fieldModes == a.fieldModes) by { assert a == b; }
+                      
+              return; 
+      }  // if a is in ks after clone -- if it got added magically...
+
+          assert xo in rm.ks;
+          assert xm != rm;
+      //    assert rr == xo;
+
+          MX := MX - rm.ks;
+          assert rm.ks > xm.ks;
+          oldmks := xm.ks;
+          oldmok := true;
+          xm := rm;
+          assert xm.ks >= m'.ks;       
+          assert xm.ks > oldmks;
+
+          assert xm.from(m');
+
+
+//          MX := a.extra - rm.ks;          
+          assert xm == rm;
+        } // end loop MX
+
+
+        assert xm == rm;
+        assert xm.ks >= m'.ks;      
+        assert a !in xm.ks;    
+        assert (a.AMFO - {a})<= xm.ks;
+        assert a.extra <= a.AMFO;
+        assert a !in a.extra;
+        assert a.extra <= (a.AMFO - {a});
+        assert a.extra <= (a.AMFO - {a}) <= xm.ks;
+        assert a.extra <= xm.ks;
+  
+        assert xm.calid(); assert rm.calid();
+        assert a.AMFO - {a} - a.extra <= rm.ks; 
+      //  SubsetOfKeysOfExtendedMap(a.AMFO , rm, m);
+        assert a.extra <= rm.ks;        
+        assert a.owners() ==  a.AMFO - {a};
+        assert a.AMFO == a.region.owner.AMFO + a.extra + {a};
+        assert a.owners() <= rm.ks;
+        assert xm.ks >= m'.ks;   
+        assert xm.from(m');
+        assert a !in xm.ks;
+
+        assert a !in xm.m.Keys by { assert a !in xm.ks; }
+        assert COK(a,xm.oHeap);
+        assert a.Ready();
+        assert a.AllOwnersAreWithinThisHeap(xm.ks);
+        assert a.owners() <= xm.ks;
+        assert (a.AMFO - {a}) <= xm.ks;
+        assert (forall oo <- (a.AMFO - {a}) :: oo in xm.m.Keys);
+      //  assert (a.region.Heap? ==> xm.m[a].region.Heap?);
+        assert (a.region.Heap? ==> a.region.owner in a.AMFO);
+        assert (a.region.Heap? ==> a.region.owner in xm.m.Keys);
+      //  assert (a.region.Heap? ==> xm.m[a.region.owner] == xm.m[a].region.owner );
+      //  assert (forall oo <- a.AMFO :: xm.m[oo] in xm.m[a].AMFO);
+        assert (a.region.Heap? ==> a.extra <= a.AMFO);
+        assert (forall xo <- a.extra :: xo in xm.m.Keys);
+      //  assert (forall xo <- a.extra :: xm.m[xo] in xm.m[a].extra) ;
+
+        assert a !in rm.ks;
+        rm.WeAreDevo();
+        assert a !in rm.vs  by { Map.AintNoSunshine(a, rm); }
+        m := rm.putOutside(a);  
         b := m.at(a);
         assert b == a;
         assert b.fieldModes == a.fieldModes;
-// 
-//             assert (b == a) by {
-//               assert not(inside(a, m.o));   //glurk
-//               assert m.AreWeNotMen(a,m);
-//               assert b == a;      //double glurk 
-//             }
 
 
-            assert m.at(a).fieldModes == a.fieldModes;
-            b := m.at(a);
-            assert b == m.m[a];
+        assert m.at(a).fieldModes == a.fieldModes;
+        b := m.at(a);
+        assert b == m.m[a];
 
-            assert (b == a) by {
-              assert not(inside(a, m.o));   //glurk
-              reveal m.AreWeNotMen();
-              assert m.AreWeNotMen(a,m);
-              assert ((not(inside(a, m.o))) ==> (m.m[a] == a));
-              assert (m.m[a] == a);
-              assert (m.m[a] == m.at(a) == a);
-              assert b == a;      //double glurk 
-            }
-
+        assert (b == a) by {
+          assert not(inside(a, m.o));   //glurk
+          reveal m.AreWeNotMen();
+          assert m.AreWeNotMen(a,m);
+          assert ((not(inside(a, m.o))) ==> (m.m[a] == a));
+          assert (m.m[a] == a);
+          assert (m.m[a] == m.at(a) == a);
+          assert b == a;      //double glurk 
+        }
 
         assert COK(b, m.oHeap);
         COKWiderContext(b, m.oHeap, m.ns);
@@ -1527,8 +2092,10 @@ assert MapOK(rm.m) && rowner.AMFO <= rm.ks;
         MapOKFromCalid(m);
         assert MapOK(m.m);
         assert mapLEQ(rm.m, m.m);
-        assert a.owners() <= rm.ks by { reveal AMFOOKRM; }
-        SubsetOfKeysOfExtendedMap(a.AMFO, rm, m);
+        assert m.from(rm);  assert m.from(m');    
+    //    assert a.owners() <= rm.ks by { reveal AMFOOKRM; }
+    assert a.AMFO - {a} - a.extra <= rm.ks; 
+  //      SubsetOfKeysOfExtendedMap(a.AMFO, rm, m);
         assert a.owners() <= m.ks;
 
         assert b.fieldModes == a.fieldModes;
@@ -1538,9 +2105,11 @@ assert MapOK(rm.m) && rowner.AMFO <= rm.ks;
 
 
 
-method {:isolate_assertions} Clone_Outside_World(a : Object, m' : Map)
+method Clone_Outside_World(a : Object, m' : Map)
       returns (b : Object, m : Map)
   decreases (m'.oHeap - m'.ks), a.AMFO, (a.fields.Keys), 15 //Clone_Outside_World
+
+  requires a.extra == {} //extra not yet cloned
 
 //this case 
   requires a !in m'.ks
@@ -1570,8 +2139,11 @@ method {:isolate_assertions} Clone_Outside_World(a : Object, m' : Map)
   ensures  m.ns >= m'.ns
 //  ensures  if (inside(a, m'.o)) then (b in m.ns) else (b == a)
 //  ensures  reveal m.calid(); reveal m.calidMap(); assert m.calid(); assert 
-  ensures MapOK(m.m) && a.owners() <= m.ks
-  
+  ensures MapOK(m.m) 
+  ensures a.AMFO <= m.ks  //seems weird but we are populating m, right...
+  ensures a.extra <= m.ks //ditto?
+  //ensures b.AMFO == set x <- a.AMFO :: m.m[x] 
+
   ensures a.fieldModes == b.fieldModes
  // ensures b.fields.Keys == a.fields.Keys
   // modifies (set o : Object | o !in (m'.oHeap+m'.ns))`fields
@@ -1655,11 +2227,15 @@ method {:isolate_assertions} Clone_Inside_Heap(a : Object, m' : Map)
   requires inside(a,m'.o)
   requires a.region.Heap?
 
+  requires a.extra == {} //extra not yet cloned
+
+
 //all Clone_
   requires m'.calid()
   requires a in m'.oHeap 
   requires COK(a, m'.oHeap)
-
+  
+  //requires CallOK(a.extra,m'.oHeap); ///now covered by the above?
 
   ensures  m.calid()
   ensures  a in m.ks
@@ -1683,10 +2259,10 @@ method {:isolate_assertions} Clone_Inside_Heap(a : Object, m' : Map)
   ensures  m.ns >= m'.ns
 //  ensures  if (inside(a, m'.o)) then (b in m.ns) else (b == a)
 //  ensures  reveal m.calid(); reveal m.calidMap(); assert m.calid(); assert 
-   ensures MapOK(m.m) && a.owners() <= m.ks
-
-
-
+  ensures MapOK(m.m) 
+  ensures a.AMFO <= m.ks  //seems weird but we are populating m, right...
+  ensures a.extra <= m.ks //ditto?
+  //ensures b.AMFO == set x <- a.AMFO :: m.m[x] 
 
    ensures b.fieldModes == a.fieldModes
 //   ensures b.fields.Keys == a.fields.Keys
@@ -1726,6 +2302,13 @@ print "VARIANT CIH ", |(m'.oHeap - m'.ks)|, " ", |a.AMFO|, " ", |(a.fields.Keys)
 
         }
 
+//makde COK check for this, no need to do another level here?
+// assert forall x <- a.extra :: COK(x,m.oHeap);
+// forall x <- a.extra ensures COK(x,m.oHeap) 
+// {
+//   assert true;
+// }   
+//assert CallOK(a.extra,m.oHeap);
 
         assert (a.region.owner.AMFO < a.AMFO) by {
             assert m.calid();
@@ -1740,8 +2323,12 @@ print "VARIANT CIH ", |(m'.oHeap - m'.ks)|, " ", |a.AMFO|, " ", |(a.fields.Keys)
             assert a.region.owner.AMFO <=  a.AMFO;
                     }
 
+
+reveal COK(); assert a.region.owner.extra == {}; //extra not yet cloned
+
         var rowner, rm := Clone_Via_Map(a.region.owner, m);
- 
+        assert rm.from(m);
+
         assert COK(rowner, rm.oHeap+rm.ns);
 
         reveal rm.calid();
@@ -1760,6 +2347,8 @@ print "VARIANT CIH ", |(m'.oHeap - m'.ks)|, " ", |a.AMFO|, " ", |(a.fields.Keys)
         assert CallOK(rm.ks, rm.oHeap);
         assert CallOK(rm.vs, rm.oHeap+rm.ns);
         assert CallOK(rm.ns, rm.oHeap+rm.ns);
+
+
 
 //should we rename oHeap as context?
 
@@ -1825,8 +2414,17 @@ assert CallOK(rm.oHeap+rm.ns);
 
 assert COK(rowner, rm.oHeap+rm.ns);
 assert CallOK(rm.oHeap+rm.ns);
+assert a.extra <= rm.oHeap by { assert COK(a, rm.oHeap); reveal COK(); }
+CallOKNarrowFocus({},rm.oHeap+rm.ns);    //WTF is this doiung?  why?
+assert CallOK({},rm.oHeap+rm.ns);        //and this one?
 
-        b := new Object.cake(a.fieldModes, rowner, rm.oHeap+rm.ns, "clone of " + a.nick);
+
+      
+        b := new Object.cake(a.fieldModes, rowner, rm.oHeap+rm.ns, "clone of " + a.nick);  // no extra
+
+        // currently ignoring REXTRA //TODO...   //extra not yet cloned
+        // var rextra := set x <- a.extra :: m.m[x];
+        // b := new Object.cake(a.fieldModes, rowner, rm.oHeap+rm.ns, "clone of " + a.nick, rextra);
 
         assert fresh(b);
         assert b.fieldModes == a.fieldModes;
@@ -1839,12 +2437,18 @@ assert CallOK(rm.oHeap+rm.ns);
         // assert COK(b, {b} + rm.oHeap+rm.m.Values);
         assert a.region.Heap? == b.region.Heap?;
 
-        assert rm.calid();
-        assert rm.calidOK();
-        assert rm.calidMap();
         reveal rm.calid();
+        reveal rm.calidObjects();        
         reveal rm.calidOK();
         reveal rm.calidMap();
+        reveal rm.calidSheep();   
+
+        assert rm.calid();
+        assert rm.calidObjects();
+        assert rm.calidOK();
+        assert rm.calidMap();
+        assert rm.calidSheep();
+
         assert COK(a,rm.oHeap);
         reveal COK();
         assert a.owners() <= rm.oHeap;
@@ -1853,12 +2457,19 @@ assert CallOK(rm.oHeap+rm.ns);
         assert COK(b, rm.oHeap+rm.ns+{b});
         assert b !in (rm.oHeap+rm.ns);
 
-        var xm := rm.putInside(a,b);  
+        assert MapOK(rm.m);
+        //assert forall kx <- a.extra :: rm.m[kx] in b.extra;   //extra not yet cloned
+
+assert a.extra == {};
+assert a.owners() <= rm.ks;
+
+
+        var xm := rm.putInside(a,b);
         assert xm.m == MappingPlusOneKeyValue(rm.m,a,b);
         
 assert xm.ks >= rm.ks + {a};
 assert xm.vs >= rm.vs + {b};
-        assert COK(b, xm.oHeap+xm.ns);
+        assert COK(b, xm.oHeap+xm.ns);  
 
         MapOKFromCalid(xm);
         assert xm.calid();
@@ -1910,19 +2521,22 @@ assert m.vs >= m'.vs + {b};
 
 
 
-method {:onlyCIW}  Clone_Inside_World(a : Object, m' : Map)
+method Clone_Inside_World(a : Object, m' : Map)
       returns (b : Object, m : Map)
   decreases (m'.oHeap - m'.ks), a.AMFO, (a.fields.Keys), 15 //Clone_Inside_World(
 
 //this case
-  requires a !in m'.ks
   requires inside(a,m'.o)
   requires a.region.World?
+  requires a !in m'.ks
 
+  requires a.extra == {} //extra not yet cloned
+  
 //all Clone_
   requires m'.calid()
   requires a in m'.oHeap 
   requires COK(a, m'.oHeap)
+
 
   ensures  m.calid()
   ensures  a in m.ks
@@ -1946,7 +2560,10 @@ method {:onlyCIW}  Clone_Inside_World(a : Object, m' : Map)
   ensures  m.ns >= m'.ns
 //  ensures  if (inside(a, m'.o)) then (b in m.ns) else (b == a)
 //  ensures  reveal m.calid(); reveal m.calidMap(); assert m.calid(); assert 
-  ensures MapOK(m.m) && a.AMFO <= m.ks
+  ensures MapOK(m.m) 
+  ensures a.AMFO <= m.ks  //seems weird but we are populating m, right...
+  ensures a.extra <= m.ks //ditto?
+  //ensures b.AMFO == set x <- a.AMFO :: m.m[x] 
 
 
    ensures b.fieldModes == a.fieldModes
@@ -1992,6 +2609,7 @@ print "VARIANT CIW ", |(m'.oHeap - m'.ks)|, " ", |a.AMFO|, " ", |(a.fields.Keys)
         assert m.calid();
 
         assert fresh(b);
+        assert b !in m.oHeap + m.ns;
         assert COK(a, m.oHeap); // by { reveal COKSTART; }
         assert COK(b, m.oHeap+{b});
         COKWiderContext(b, m.oHeap+{b}, m.ns);
@@ -2024,7 +2642,7 @@ print "VARIANT CIW ", |(m'.oHeap - m'.ks)|, " ", |a.AMFO|, " ", |(a.fields.Keys)
         assert mx.calidMap();
         assert MapOK(mx.m);
 
-        assert a.AMFO == {};
+        assert a.AMFO == {a};
         assert a.AMFO <= mx.ks;
 
         m := Clone_All_Fields(a,b, mx);
@@ -2175,6 +2793,8 @@ assert m.calid();
 
 label B3:
 assert m.calid();
+
+reveal COK(); assert ofv.extra == {}; //extra not yet cloned
 
     var rfv, rm := Clone_Via_Map(ofv, m);
 
@@ -2419,13 +3039,305 @@ assert old@B4(CallOK(m.ns, m.oHeap+m.ns));
       assert m.calid();
 
     }
-} //end Clone_Field_Map
+} //end Clone: /_Field_Map
+
+function mapThruMap(os: set<Object>, m : Map) : set<Object>
+  reads m.oHeap`fields, m.oHeap`fieldModes
+  reads m.ns`fields, m.ns`fieldModes      
+  requires m.calid()
+  requires os <= m.ks
+  requires os <= m.m.Keys
+{
+  reveal m.calid();
+  set o <- os :: m.m[o]
+}
 
 
 
-
-
-
+// method Clone_Extra_Owners(a : Object,  m' : Map)  returns (m : Map) 
+//    
+//   decreases (m'.oHeap - m'.ks), a.AMFO, (a.fields.Keys), 12
+// 
+//   requires a.extra == {} //extra not yet cloned
+// 
+//   requires m'.calid()
+//   requires a !in m'.ks     //can we just reply on clone to do the RIGHT THING
+//   requires a in m'.oHeap 
+//   requires COK(a, m'.oHeap)
+// 
+//   // ensures  m.calid()
+//   // ensures  a.extra <= m.ks
+//   // ensures  a.extra <= m.m.Keys
+//   // ensures  && (a.extra <= m.ks)
+//   //          && (a.extra <= m.m.Keys)
+//   //          && mapThruMap(a.extra, m) <= m.vs
+// {
+//         var rm := m';
+//         var b : Object; 
+// 
+// 
+// 
+//         assert a !in rm.ks;
+//         assert a !in rm.vs by { 
+//           
+//           
+//     //            assert not(inside(a,rm.o));
+//     //            assert a !in rm.m.Keys;
+//                 assert rm.calid(); 
+//                 rm.WeAreDevo();
+//                 assert forall k <- rm.m.Keys :: rm.AreWeNotMen(k,rm);
+//                 assert a  in rm.oHeap;
+//                 assert a !in rm.ns;
+//           
+//           
+//           
+//           Map.AintNoSunshine(a, rm);
+//           assert a !in rm.vs; }
+//         assert rm.ks >= m'.ks;
+//         assert mapLEQ(m'.m,rm.m);
+//         assert rm.from(m');
+// 
+// //    //maintaing MapOK
+// //         assert AMFOOKRM: a.owners() <= rm.ks by {
+// //             reveal rm.calid();
+// //             assert rm.calid();
+// //             reveal rm.calidMap();
+// //             assert rm.calidMap();
+// //             assert MapOK(rm.m);
+// //             reveal rm.calidObjects();
+// //             assert rm.calidObjects();             
+// //             assert (forall x <- rm.ks, oo <- x.AMFO :: oo in rm.ks);
+// //             assert a.owners() <= rm.ks by {
+// //                reveal COK(); 
+// //                assert COK(a,m.oHeap); 
+// //                assert a.AMFO <= m.oHeap;
+// // //               assert a.owners() <= rm.ks;
+// //                }
+// //         }
+// 
+// 
+// 
+//         assert a in rm.oHeap; 
+//         assert COK(a, rm.oHeap);
+//         reveal COK();
+//         assert a.AMFO <= rm.oHeap;
+//       //  assert a.owners() <= rm.ks;
+//       if (outside(a,rm.o)) {
+//         OutsidersArentMapValues(a,rm);
+//         assert a !in rm.vs;
+//         assert a !in rm.ks;
+//         assert not(inside(a, rm.o)); 
+//       }
+// 
+//         //m := rm[a:=b];     
+// 
+// 
+//         assert COK(a, rm.oHeap);
+// 
+//         assert rm.calid();
+//         assert a in rm.oHeap;
+//         assert COK(a, rm.oHeap);
+//         assert a.extra <= rm.oHeap; 
+// 
+//         assert CallOK(rm.oHeap) by {
+//           reveal rm.calid(), rm.calidOK();
+//           assert rm.calid();
+//           assert rm.calidOK();
+//           reveal CallOK(), COK();
+//           assert CallOK(rm.oHeap);
+//         }
+// 
+// 
+//         var xm := rm;
+//         assert xm.ks >= m'.ks;
+//         assert mapLEQ(m'.m,xm.m);    
+//         assert xm.from(rm);
+//         assert xm.from(m');
+// 
+//         assert a !in xm.ks;
+//         assert a !in xm.vs;
+// 
+// 
+//         var MX := a.extra - xm.ks;
+//         assert MX <= a.extra;
+//         var xo : Object;
+//         var rr : Object;
+//         var oldmks  : set<Object>;  //dont fucking ask
+//         var oldmok :=  false;
+// 
+//         assert !oldmok;
+//         assert xm == rm;
+//         assert xm.ks >= (m'.ks);
+//         assert mapLEQ(m'.m,xm.m);    
+//         assert xm.from(m');
+// 
+//         assert a !in xm.ks;
+// 
+//         while ((MX != {}) && (a !in xm.ks))
+//           decreases MX
+//           invariant MX == a.extra - xm.ks
+//           invariant MX <= a.extra
+//           invariant xm == rm
+//           invariant xm.calid()
+//           invariant rm.calid()
+//           invariant m'.calid()
+//           invariant xm.from(m')  
+//           invariant MX <= xm.oHeap            
+//           invariant CallOK(xm.oHeap)    
+//           invariant a.AMFO - {a} <= xm.ks + MX
+//           invariant a.extra <= a.AMFO
+//           invariant oldmok ==> assigned(oldmks)
+//           invariant oldmok ==> (xm.ks > oldmks)
+//           invariant m'.oHeap == xm.oHeap
+//           invariant oldmok ==> ((m'.oHeap - oldmks) > (xm.oHeap - xm.ks))
+//           invariant xm.ks >= (m'.ks)
+//           invariant xm.vs >= (m'.vs)
+//           invariant a !in xm.ks
+//         {
+//           assert xm == rm;
+//           xo :| xo in MX;
+//           assert xo in MX;
+//           MX := MX - {xo};
+//            
+//           assert xm.calid();
+//           assert xo in xm.oHeap;
+//           COKfromCallOK(xo,xm.oHeap);
+//           assert COK(xo,xm.oHeap);
+//           assert xo !in xm.ks;
+//         
+//         
+//           assert oldmok ==> (m'.oHeap - oldmks) > (xm.oHeap - xm.ks);
+// 
+// assert xo in a.AMFO;
+// assert a.Ready();
+// assert xo in a.extra;
+// assert a.AMFO > xo.AMFO;
+// 
+// 
+//           assert (m'.oHeap) == m'.oHeap == xm.oHeap;
+//           assert xm.ks >= (m'.ks);
+//           assert xm.from(m');
+// 
+//   assert  mapLEQ(m'.m,xm.m) by 
+//                { reveal xm.calid(); assert xm.calid();
+//                  reveal xm.calidObjects(); assert xm.calidObjects();
+//                  assert m'.ks <= xm.ks;
+//                  assert m'.vs <= xm.vs; 
+//                  assert m'.ks == m'.m.Keys;
+//                  assert m'.vs == m'.m.Values;       
+//                  assert xm.ks == xm.m.Keys;
+//                  assert xm.vs == xm.m.Values;                              
+//                  assert m'.m.Keys <= xm.m.Keys;
+//                  assert m'.m.Values <= xm.m.Values;
+//                  assert forall k <- m'.m.Keys :: k in xm.m.Keys;
+//       assert forall k <- m'.m.Keys :: k in xm.m.Keys && (m'.m[k] == xm.m[k]);
+//                 }
+//         
+// 
+//                   assert xm.ks >= m'.ks;
+//                 assert a !in xm.ks;          
+// 
+//           assert ((m'.oHeap - m'.ks)) >= (xm.oHeap - xm.ks);
+// 
+// assert  ((a.AMFO)
+//   decreases to
+//         (xo.AMFO));
+//       
+//         assert ((m'.oHeap - m'.ks), 
+//                (a.AMFO),
+//                (a.fields.Keys), 
+//                (15) 
+//           decreases to 
+//                xm.oHeap - xm.ks, 
+//                xo.AMFO, 
+//                xo.fields.Keys, 
+//                20);
+// 
+//       
+//           rr, rm := Clone_Via_Map(xo, xm);
+//           assert rm.ks >= m'.ks;
+//           assert mapLEQ(m'.m,rm.m);    
+//           assert rm.from(m');
+// 
+//       if (a in rm.ks) { 
+//                 m := rm;
+//                 assert m.calidObjects() by {  reveal m.calid(); assert  m.calid();  }
+//                 assert  a in m.ks by { reveal m.calidObjects(); assert m.calidObjects(); }
+//                 assert  a in m.m.Keys by { reveal m.calidObjects(); assert m.calidObjects(); }
+//                 b := m.m[a];
+//                 //
+// 
+//                 assert  b in m.vs by { reveal m.calidObjects(); assert m.calidObjects();  assert b in m.m.Values; }
+//                 assert  b in m.m.Values by { reveal m.calidObjects(); assert m.calidObjects(); }
+//                 assert m.calidOK() by {  reveal m.calid(); assert  m.calid();  }
+//                 assert  a in m.m.Keys && m.at(a) == b; 
+//                 assert  COK(b, m.oHeap+m.ns) by {
+//                 assert b in m.vs;
+//                 assert CallOK(m.vs, m.oHeap+m.ns) by { reveal m.calidOK(); }
+//                 COKfromCallOK(b, m.vs, m.oHeap+m.ns);   }
+// 
+//                 assert m.from(m');
+// 
+//                 assert  mapLEQ(m'.m,m.m) by 
+//                         { reveal m.calidObjects(); assert m.calidObjects();
+//                           assert m'.ks <= m.ks;
+//                           assert mapLEQ(m'.m,m.m);    
+//                           assert m'.m.Keys <= m.m.Keys;
+//                           assert m'.m.Values <= m.m.Values;
+//                           }
+//                 assert  m.ks >= m'.ks + {a} by { reveal m.calidObjects(); assert m.calidObjects(); }
+//                 assert  m.vs >= m'.vs + {b} by { reveal m.calidObjects(); assert m.calidObjects(); }
+//                 assert  m.o == m'.o;
+//                 assert  m.oHeap == m'.oHeap;
+//                 assert  m.ns >= m'.ns;
+//                 assert MapOK(m.m);
+//                 assert forall x <- m.m.Keys, oo <- x.AMFO :: oo in m.m.Keys;
+//                 assert  a in m.m.Keys;
+//                 assert forall oo <- a.AMFO :: oo in m.m.Keys;
+//                 assert a.AMFO <= m.m.Keys;
+//                 assert m.ks == m.m.Keys by { reveal m.calidObjects(); assert m.calidObjects(); }
+//                 assert a.AMFO <= m.ks;
+//                 assert a.extra <= m.ks;
+// 
+// 
+//             
+//                 assert  a == b by {
+//                       reveal m.calid();
+//                       assert m.calidMap();
+//                       reveal m.calidMap();
+//                   //    assert (forall x <- m.ks :: (not(inside(x,m.o)) ==> (m.m[x] == x)));
+//                       assert not(inside(a,m.o));
+//                       assert m.m[a] == a;
+//                       assert a == b;
+//                   }
+// 
+//              assert (b.fieldModes == a.fieldModes) by { assert a == b; }
+//                       
+//               return; 
+//       }  // if a is in ks after clone -- if it got added magically...
+// 
+//           assert xo in rm.ks;
+//           assert xm != rm;
+//       //    assert rr == xo;
+// 
+//           MX := MX - rm.ks;
+//           assert rm.ks > xm.ks;
+//           oldmks := xm.ks;
+//           oldmok := true;
+//           xm := rm;
+//           assert xm.ks >= m'.ks;       
+//           assert xm.ks > oldmks;
+// 
+//           assert xm.from(m');
+// 
+// 
+// //          MX := a.extra - rm.ks;          
+//           assert xm == rm;
+//         } // end loop MX
+// 
+// }
+// 
+// 
 
 
 
@@ -2470,7 +3382,7 @@ lemma  OutsidersArentMapValues(a : Object, m : Map)
   if (a in m.vs) {
     AValueNeedsAKey(a,m.m);
     
-    assert not(outside(a,m.o));
+    assert {:contradiction} not(outside(a,m.o));
     assert {:contradiction} false;
   }
 }
